Veritas.BinTreePtr.fsti
@@ -8,24 +8,35 @@ open Veritas.BinTree
  *)
 type ptrfn = (n:bin_tree_node) -> (c:bin_tree_dir) -> option (d:bin_tree_node{is_desc d (child c n)})
 
-(* Is d descendant of a following pf pointers *)
-val is_pdesc (pf: ptrfn) (d a: bin_tree_node): Tot bool
+(* Is d reachable from a following pf pointers *)
+val reachable (pf: ptrfn) (d a: bin_tree_node): Tot bool
 
-(* are a1 a2 in anc-desc relationship wrt p *)
-let is_panc_pdesc_sym (pf: ptrfn) (a1 a2: bin_tree_node): bool = 
-  is_pdesc pf a1 a2 || is_pdesc pf a2 a1
+(* is reachable from the root *)
+let root_reachable (pf: ptrfn) (n: bin_tree_node): bool = reachable pf n Root
+
+(* are a1 a2 reachable from one or the other *)
+let reachable_sym (pf: ptrfn) (a1 a2: bin_tree_node): bool = 
+  reachable pf a1 a2 || reachable pf a2 a1
 
 (* unrelated in terms of p-anc-desc *)
-let non_panc_pdesc (pf: ptrfn) (a1 a2: bin_tree_node): bool = 
-  not (is_panc_pdesc_sym pf a1 a2)
+let non_reachable_sym (pf: ptrfn) (a1 a2: bin_tree_node): bool = 
+  not (reachable_sym pf a1 a2)
 
 (* every node is a pdesc of itself *)
-val lemma_pdesc_reflexive (pf: ptrfn) (a: bin_tree_node):
-  Lemma (is_pdesc pf a a)
+val lemma_reachable_reflexive (pf: ptrfn) (a: bin_tree_node):
+  Lemma (reachable pf a a)
 
 (* pdesc is a transitive relation *)
-val lemma_pdesc_transitive (pf: ptrfn) (a b c: bin_tree_node):
-  Lemma (requires (is_pdesc pf a b /\ is_pdesc pf b c))
-        (ensures (is_pdesc pf a c))
+val lemma_reachable_transitive (pf: ptrfn) (a b c: bin_tree_node):
+  Lemma (requires (reachable pf a b /\ reachable pf b c))
+        (ensures (reachable pf a c))
 
-
+(* 
+ * if there is no c-pointer at node a, then any desc in that subtree is not 
+ * reachable from a 
+ *)
+val non_reachable_desc_of_none (pf: ptrfn) 
+                               (d:bin_tree_node) 
+                               (a:bin_tree_node{is_proper_desc d a /\ 
+                                                None? (pf a (desc_dir d a))}):
+  Lemma (not (reachable pf d a))
